feat(*) now really added the final missing files...

HOL_To_IMP_Minus/Refinements/HOL_To_IMP_Minus_Datatypes.thy
@@ -17,19 +17,10 @@ end
 context HOL_Nat_To_IMP_Minus
 begin
 
+thm Pair_nat_def
 compile_nat Pair_nat_def
 HOL_To_IMP_Minus_correct Pair_nat by cook
 
-lemmas fst_nat_eq_unfolded = HTHN.fst_nat_eq_unfolded[simplified case_prod_nat_def]
-unconditional_nat fst_nat_eq_unfolded
-declare fst_nat_unconditional.simps[simp del]
-compile_nat fst_nat_unconditional.simps
-HOL_To_IMP_Minus_correct fst_nat_unconditional by cook
-
-(* Problem: We have obtained an unconditional equation. However, we
-still have to prove it to be related to the original HOL function.
-TODO: how to prove the two functions to be related? Currently, we are
-missing the right lemmas to make it automatic. *)
 context
   fixes xs and xs' :: "'a :: compile_nat * 'b :: compile_nat"
   assumes rels: "Rel_nat xs xs'"
@@ -38,12 +29,6 @@ begin
   print_statement HTHN.fst_nat_eq_unfolded
   print_statement HTHN.fst_nat_eq_unfolded[OF rels, unfolded case_list_nat_def]
 end
-
-lemmas snd_nat_eq_unfolded = HTHN.snd_nat_eq_unfolded[simplified case_prod_nat_def]
-unconditional_nat snd_nat_eq_unfolded
-declare snd_nat_unconditional.simps[simp del]
-compile_nat snd_nat_unconditional.simps
-HOL_To_IMP_Minus_correct snd_nat_unconditional by cook
 
 end
 
@@ -62,6 +47,7 @@ lemma rev_acc_eq_rev_append [simp]: "rev_acc xs ys = List.rev xs @ ys"
 
 case_of_simps rev_acc_eq : rev_acc.simps
 function_compile_nat rev_acc_eq
+print_theorems
 
 end
 
@@ -76,121 +62,299 @@ HOL_To_IMP_Minus_correct Nil_nat by cook
 
 (* FIXME: we could use the equation without unfolding case_list_nat_def if we prove
 congruence lemmas for case_list_nat (otherwise the function package cannot prove termination) *)
-lemmas rev_acc_nat_eq = HTHN.rev_acc_nat_eq_unfolded[simplified case_list_nat_def]
-unconditional_nat rev_acc_nat_eq
-declare rev_acc_nat_unconditional.simps[simp del]
-compile_nat rev_acc_nat_unconditional.simps
-HOL_To_IMP_Minus_correct rev_acc_nat_unconditional by (cook mode = tailcall)
+lemmas rev_acc_nat_eq = HOL_To_HOL_Nat.rev_acc_nat_eq_unfolded[simplified case_list_nat_def]
+compile_nat rev_acc_nat_eq
 
-(*Manual attempt to prove the relatedness to HOL function*)
-lemma natify_list_simps_Nil: "natify [] = Nil_nat"
-  by (subst natify_list.simps) simp
+thm eq_if_natify_eq
+(*automatically generated theorems*)
+thm Rel_nat_destruct_Cons
+thm HOL_To_HOL_Nat_Basics.Rel_nat_list
+thm Rel_nat_compile_nat
+lemmas fst_nat_eq_if_Rel_nat_list = rel_funD[OF Rel_nat_eq_fst_nat_case_list]
+thm Rel_nat_eq_fst_nat_case_list
 
-lemma natify_list_simps_Cons: "natify (x # xs) = Cons_nat (natify x) (natify xs)"
-  by (subst natify_list.simps) simp
+lemma check_first_nat_ccontradictionE:
+  assumes "fst_nat n = m"
+  and "fst_nat n = k"
+  obtains "fst_nat n = m" "k = m"
+  using assms by simp
 
-(* we would need these elimination/destruction lemmas to automate the proofs *)
-lemma Rel_nat_NilE:
-  assumes rel: "Rel_nat xs []"
-  obtains "xs = Nil_nat"
-  (* this proof is not "optimal", but can hopefully be mechanically derived for each constructor *)
-  apply standard
-  apply (subst rel[simplified Rel_nat_iff_eq_natify])
-    apply (subst natify_list_simps_Nil)
-    apply (rule refl)
-   apply ((rule Rel_nat_natify_self)+)?
-  done
+lemma check_first_nat_ccontradictionE':
+  assumes "fst_nat n \<noteq> m"
+  and "fst_nat n = k"
+  obtains "fst_nat n \<noteq> m" "k \<noteq> m"
+  using assms by simp
 
-lemma Rel_nat_ConsE:
-  assumes rel: "Rel_nat xs (y # ys)"
-  obtains z zs where "xs = Cons_nat z zs" "Rel_nat z y" "Rel_nat zs ys"
-  apply standard
-  apply (subst rel[simplified Rel_nat_iff_eq_natify])
-    apply (subst natify_list_simps_Cons)
-    apply (rule refl)
-   apply ((rule Rel_nat_natify_self)+)?
-  done
+(*
+Save reference to eq_unfolded in Symtab (\<rightarrow> under long name),
+When saving in Termtab the types are instantiated weirdly
+and the thm is not found
+*)
 
-lemma Rel_nat_NilD:
-  assumes "Rel_nat xs []"
-  shows "xs = Nil_nat"
-  using assms Rel_nat_NilE by blast
+HOL_To_IMP_Minus_correct HOL_To_HOL_Nat.rev_acc_nat
+  oops
 
-lemma Rel_nat_ConsD:
-  assumes "Rel_nat xs (y # ys)"
-  shows "\<exists>z zs. xs = Cons_nat z zs \<and> Rel_nat z y \<and> Rel_nat zs ys"
-  using assms Rel_nat_ConsE by blast
+(* Findings:
+ - For introduction over multiple variable we need to apply the search for
+    contradiction multiple times
+ - Problem mit if-placement siehe count_acc Beispiel *)
 
-(* probably(?) best approach: use induction on the original function's definition *)
-lemma related_rev_acc_nat_unconditional:
-  fixes xs acc and xs' acc' :: "('a :: compile_nat) list"
-  assumes rels: "Rel_nat xs xs'" "Rel_nat acc acc'"
-  shows "Rel_nat (rev_acc_nat_unconditional xs acc) (HTHN.rev_acc xs' acc')"
-  using assms
-  apply (induction xs' acc' arbitrary: xs acc rule: HTHN.rev_acc.induct)
+lemma rev_acc_cor:
+  assumes "Rel_nat (s ''rev_acc_nat.args.x'') (x :: 'a list)"
+  assumes "Rel_nat (s ''rev_acc_nat.args.xa'') (xa :: 'a list)"
+  shows "terminates_with_res_IMP_Minus (tailcall_to_IMP_Minus rev_acc_nat_IMP_tailcall) s ''rev_acc_nat.ret''
+    (HTHN.rev_acc_nat TYPE('a :: compile_nat) (s ''rev_acc_nat.args.x'') (s ''rev_acc_nat.args.xa''))"
+  using assms apply -
+  apply (rule terminates_with_res_IMP_Minus_if_terminates_with_res_IMP_TailcallI)
+    apply (subst rev_acc_nat_IMP_tailcall_def; simp)
+  apply (subst rev_acc_nat_IMP_tailcall_def; simp)
+  apply (induction "x" "xa" arbitrary: s rule: HTHN.rev_acc.induct)
+  (*case []*)
+  apply (subst (2) rev_acc_nat_IMP_tailcall_def, rule terminates_with_res_IMP_Tailcall_start)
+   apply (tactic \<open>HT.run_step_tac HT.get_imp_minus_correct @{context} 1\<close>)+
+    (*check the retrieved condition for a contradiction (needs to be built into the IF tactic*)
+    apply (erule check_first_nat_ccontradictionE check_first_nat_ccontradictionE')
+    apply (rule fst_nat_eq_if_Rel_nat_list)
+    apply assumption (*needs a smarter method*)
+    apply simp
+  apply (subst HTHN.rev_acc_nat_eq_unfolded)
+  apply (assumption, assumption)
+  apply (subst case_list_nat_def)
+  apply (split if_splits; intro impI conjI; simp)
+  apply (tactic \<open>HT.finish_non_tail_tac @{context} 1\<close>)
+    (*we need to derive a contradiction*)
+    apply (erule check_first_nat_ccontradictionE check_first_nat_ccontradictionE')
+    apply (rule fst_nat_eq_if_Rel_nat_list)
+    apply assumption
+    apply simp
+  (*case x#xs*)
+  apply (subst (2) rev_acc_nat_IMP_tailcall_def, rule terminates_with_res_IMP_Tailcall_start)
+  apply (tactic \<open>HT.run_step_tac HT.get_imp_minus_correct @{context} 1\<close>)+
+    (*we need to derive a contradiction*)
+    apply (erule check_first_nat_ccontradictionE check_first_nat_ccontradictionE')
+    apply (rule fst_nat_eq_if_Rel_nat_list)
+    apply assumption
+    apply simp
+    (*check the retrievied condition for a contradiction*)
+    apply (erule check_first_nat_ccontradictionE check_first_nat_ccontradictionE')
+    apply (rule fst_nat_eq_if_Rel_nat_list)
+    apply assumption
+    apply simp
+  apply (tactic \<open>HT.run_step_tac HT.get_imp_minus_correct @{context} 1\<close>)+
 
-  apply (subst HTHN.rev_acc.simps)
-  apply (frule Rel_nat_NilD Rel_nat_ConsD; (elim exE)?)
-  apply hypsubst
-  apply (subst rev_acc_nat_unconditional.simps)
-  apply (simp (no_asm) add: Nil_nat_def Cons_nat_def,
-   (simp (no_asm) only: flip: Nil_nat_def Cons_nat_def)?)
+  apply (tactic \<open>HT.finish_tail_tac @{context} 1\<close>)
 
-  apply (subst HTHN.rev_acc.simps)
-  apply (frule Rel_nat_NilD Rel_nat_ConsD; (elim conjE exE)?)
-  apply hypsubst
-  apply (subst rev_acc_nat_unconditional.simps)
-  apply (simp (no_asm) add: Nil_nat_def Cons_nat_def,
-   (simp (no_asm) only: flip: Nil_nat_def Cons_nat_def)?)
-  subgoal premises p
-    apply (urule p(1))
-    apply (insert p(2-))
-    apply (metis Rel_nat_Cons_nat rel_funD)
-    apply (metis Rel_nat_Cons_nat rel_funD)
-    done
-  done
+  apply (subst HTHN.rev_acc_nat_eq_unfolded)
+  apply (assumption, assumption)
+   apply (subst case_list_nat_def)
+  apply (split if_splits; intro impI conjI; simp)
+  (*apply IH; prove side-conditions*)
+  sorry
+
+HOL_To_IMP_Minus_correct HOL_To_HOL_Nat.rev_acc_nat
+  using rev_acc_cor by blast
+
+ML \<open>
+val _ = @{print} @{term "TYPE ('a)"}
+\<close>
 
 end
 
 context HOL_To_HOL_Nat
 begin
+definition "rev2 xs \<equiv> rev_acc xs []"
+function_compile_nat rev2_def
+print_theorems
 
-lemma rev_eq_rev_acc_nil: "List.rev xs = rev_acc xs []" by simp
+lemma rev_acc_Nil_Nil: "rev_acc [] [] = []"
+  by simp
 
-end
+fun rev_test :: "'a list \<Rightarrow> nat list" where
+  "rev_test [] = (if rev_acc [] ([]::'a list) = [] then [] else [Suc 0])"
+| "rev_test xs = (if rev_acc xs [] = [] then [] else [Suc (Suc 0)])"
+declare rev_acc.simps[simp del]
+(* Try around with this function *)
 
-experiment
-begin
-interpretation HOL_To_HOL_Nat .
-function_compile_nat rev_eq_rev_acc_nil
-(*We couldn't use 'unconditional_nat' this way since the synthesised definition uses an auxiliary
-function (rev_acc_nat) with TYPE('a) arguments.*)
-print_statement rev_nat_eq_unfolded
-end
+case_of_simps rev_test_eq : rev_test.simps
+function_compile_nat rev_test_eq
+print_theorems
 
-context HOL_To_HOL_Nat
-begin
-
-(*we can fix this by registering the relatedness theorem of the unconditional rev_acc_nat function
-to transfer instead*)
-declare HNTIM.related_rev_acc_nat_unconditional[transfer_rule]
-  and rev_acc_related_transfer[transfer_rule del] (*deletion is optional*)
-function_compile_nat rev_eq_rev_acc_nil
-print_statement rev_nat_eq_unfolded
 end
 
 context HOL_Nat_To_IMP_Minus
 begin
 
-unconditional_nat HTHN.rev_nat_eq_unfolded
-declare rev_nat_unconditional.simps[simp del]
-compile_nat rev_nat_unconditional.simps
-HOL_To_IMP_Minus_correct rev_nat_unconditional by cook
+compile_nat HOL_To_HOL_Nat.rev2_nat_eq_unfolded
 
-(*TODO: derive these theorems automatically*)
-lemma related_rev_nat_unconditional [transfer_rule]:
-  "(Rel_nat ===> Rel_nat) rev_nat_unconditional rev"
+declare [[show_types]]
+declare HTHN.rev2_nat_eq_unfolded[]
+
+HOL_To_IMP_Minus_correct HOL_To_HOL_Nat.rev2_nat
+  apply (rule terminates_with_res_IMP_Minus_if_terminates_with_res_IMP_TailcallI)
+  apply (subst rev2_nat_IMP_tailcall_def; simp)
+  apply (subst rev2_nat_IMP_tailcall_def; simp)
+    (* No induction for defs *)
+  apply (subst (2) rev2_nat_IMP_tailcall_def, rule terminates_with_res_IMP_Tailcall_start)
+  apply (tactic \<open>HT.run_step_tac HT.get_imp_minus_correct @{context} 1\<close>)
+  apply (tactic \<open>HT.run_step_tac HT.get_imp_minus_correct @{context} 1\<close>)
+  apply (tactic \<open>HT.run_step_tac HT.get_imp_minus_correct @{context} 1\<close>)
+  apply (tactic \<open>HT.run_step_tac HT.get_imp_minus_correct @{context} 1\<close>)
+  apply (tactic \<open>HT.run_step_tac HT.get_imp_minus_correct @{context} 1\<close>)
+  by (tactic \<open>HT.finish_non_tail_tac @{context} 1\<close>)
+
+(* FIXME: we could use the equation without unfolding case_list_nat_def if we prove
+congruence lemmas for case_list_nat (otherwise the function package cannot prove termination) *)
+lemmas rev_test_nat_eq = HOL_To_HOL_Nat.rev_test_nat_eq_unfolded[simplified case_list_nat_def]
+compile_nat rev_test_nat_eq
+
+HOL_To_IMP_Minus_correct HOL_To_HOL_Nat.rev_test_nat
+  apply (rule terminates_with_res_IMP_Minus_if_terminates_with_res_IMP_TailcallI)
+    apply (subst rev_test_nat_IMP_tailcall_def; simp)
+   apply (subst rev_test_nat_IMP_tailcall_def; simp)
+  apply (induction y arbitrary: s rule: HTHN.rev_test.induct)
+  (* case [] *)
+  apply (subst (2) rev_test_nat_IMP_tailcall_def, rule terminates_with_res_IMP_Tailcall_start)
+  apply (tactic \<open>HT.run_step_tac HT.get_imp_minus_correct @{context} 1\<close>)
+  apply (tactic \<open>HT.run_step_tac HT.get_imp_minus_correct @{context} 1\<close>)
+  apply (tactic \<open>HT.run_step_tac HT.get_imp_minus_correct @{context} 1\<close>)
+  apply (tactic \<open>HT.run_step_tac HT.get_imp_minus_correct @{context} 1\<close>)
+  apply (tactic \<open>HT.run_step_tac HT.get_imp_minus_correct @{context} 1\<close>)
+  apply (tactic \<open>HT.run_step_tac HT.get_imp_minus_correct @{context} 1\<close>)
+  apply (tactic \<open>HT.run_step_tac HT.get_imp_minus_correct @{context} 1\<close>)
+  apply (tactic \<open>HT.run_step_tac HT.get_imp_minus_correct @{context} 1\<close>)
+  subgoal for s
+    apply (tactic \<open>HT.run_step_tac HT.get_imp_minus_correct @{context} 1\<close>)
+    apply (tactic \<open>HT.run_step_tac HT.get_imp_minus_correct @{context} 1\<close>)
+    apply (tactic \<open>HT.run_step_tac HT.get_imp_minus_correct @{context} 1\<close>)
+    apply (tactic \<open>HT.run_step_tac HT.get_imp_minus_correct @{context} 1\<close>)
+    (* unwanted TYPE variable is introduced *)
+    apply (tactic \<open>HT.run_step_tac HT.get_imp_minus_correct @{context} 1\<close>)
+    apply (tactic \<open>HT.run_step_tac HT.get_imp_minus_correct @{context} 1\<close>)
+    apply (tactic \<open>HT.run_step_tac HT.get_imp_minus_correct @{context} 1\<close>)
+    apply (tactic \<open>HT.run_step_tac HT.get_imp_minus_correct @{context} 1\<close>)
+    apply (tactic \<open>HT.run_step_tac HT.get_imp_minus_correct @{context} 1\<close>)
+    apply (tactic \<open>HT.run_step_tac HT.get_imp_minus_correct @{context} 1\<close>)
+    apply (tactic \<open>HT.run_step_tac HT.get_imp_minus_correct @{context} 1\<close>)
+    apply (tactic \<open>HT.run_step_tac HT.get_imp_minus_correct @{context} 1\<close>)
+
+    apply (tactic \<open>HT.finish_non_tail_tac @{context} 1\<close>)
+
+    apply (subst HTHN.rev_test_nat_eq_unfolded)
+    apply (tactic \<open>HOL_Nat_To_IMP_Tactics_Base.transfer_foc_rev_tac @{context} 1\<close>)
+
+     apply (subst case_list_nat_def)
+     apply (simp only: split: if_splits)
+     apply (intro conjI impI)
+            apply simp
+    apply simp
+    apply simp
+         apply simp
+    defer
+        apply simp
+    subgoal
+      sorry
+    apply auto[]
+    apply simp
+
+
+    (* Apply transfer here *)
+    subgoal
+      sorry
+
+    apply (tactic \<open>HT.run_step_tac HT.get_imp_minus_correct @{context} 1\<close>)
+    apply (tactic \<open>HT.run_step_tac HT.get_imp_minus_correct @{context} 1\<close>)
+    apply (tactic \<open>HT.run_step_tac HT.get_imp_minus_correct @{context} 1\<close>)
+    apply (tactic \<open>HT.run_step_tac HT.get_imp_minus_correct @{context} 1\<close>)
+    apply (tactic \<open>HT.run_step_tac HT.get_imp_minus_correct @{context} 1\<close>)
+    apply (tactic \<open>HT.run_step_tac HT.get_imp_minus_correct @{context} 1\<close>)
+    apply (tactic \<open>HT.finish_non_tail_tac @{context} 1\<close>)
+    (* First apply transfer then find a contradiction *)
+
+    (* stupid sledgehammer: *)
+    using Rel_nat_Nil_nat fst_nat_eq_if_Rel_nat_list rev_acc_nat_eq
+    by force
+
+    (* Find contradiction *)
+    apply (erule check_first_nat_ccontradictionE check_first_nat_ccontradictionE')
+    apply (rule fst_nat_eq_if_Rel_nat_list)
+    apply assumption (*needs a smarter method*)
+   apply simp
+  (* case (_#_) *)
+  apply (subst (2) rev_test_nat_IMP_tailcall_def, rule terminates_with_res_IMP_Tailcall_start)
+  apply (tactic \<open>HT.run_step_tac HT.get_imp_minus_correct @{context} 1\<close>)+
+    (* Find contradiction *)
+    apply (erule check_first_nat_ccontradictionE check_first_nat_ccontradictionE')
+    apply (rule fst_nat_eq_if_Rel_nat_list)
+    apply assumption (*needs a smarter method*)
+    apply simp
+  subgoal for x xs s
+    apply (tactic \<open>HT.run_step_tac HT.get_imp_minus_correct @{context} 1\<close>)
+    apply (tactic \<open>HT.run_step_tac HT.get_imp_minus_correct @{context} 1\<close>)
+    apply (tactic \<open>HT.run_step_tac HT.get_imp_minus_correct @{context} 1\<close>)
+    apply (tactic \<open>HT.run_step_tac HT.get_imp_minus_correct @{context} 1\<close>)
+    apply (tactic \<open>HT.run_step_tac HT.get_imp_minus_correct @{context} 1\<close>)
+    apply (tactic \<open>HT.run_step_tac HT.get_imp_minus_correct @{context} 1\<close>)
+    apply (tactic \<open>HT.run_step_tac HT.get_imp_minus_correct @{context} 1\<close>)
+    apply (tactic \<open>HT.run_step_tac HT.get_imp_minus_correct @{context} 1\<close>)
+    apply (tactic \<open>HT.run_step_tac HT.get_imp_minus_correct @{context} 1\<close>)
+    apply (tactic \<open>HT.run_step_tac HT.get_imp_minus_correct @{context} 1\<close>)
+    apply (tactic \<open>HT.run_step_tac HT.get_imp_minus_correct @{context} 1\<close>)
+    apply (tactic \<open>HT.run_step_tac HT.get_imp_minus_correct @{context} 1\<close>)
+    apply (tactic \<open>HT.run_step_tac HT.get_imp_minus_correct @{context} 1\<close>)
+    apply (tactic \<open>HT.run_step_tac HT.get_imp_minus_correct @{context} 1\<close>)
+
+    (* Do step tac for tCall manually *)
+    (* Split tSeq *)
+    apply (tactic \<open>HOL_Nat_To_IMP_Tailcalls_Tactics.terminates_with_res_tSeq_tac @{context} 1\<close>)
+
+    (* Apply tCall rule and apply correctness \<rightarrow> need to proof Rel_nat(s) *)
+    apply (rule terminates_with_tCallI)
+      apply (rule rev_acc_nat_IMP_Minus_imp_minus_correct)
+
+
+  apply (rule Rel_nat_rewrite_lhs)
+  apply (tactic \<open>SUT.STATE_interp_retrieve_key_eq_tac (simp_tac @{context}) @{context} 1\<close>)
+  apply (tactic \<open>HOL_Nat_To_IMP_Minus_Tactics_Base.transfer_foc_rev_tac @{context} 1\<close>)
+
+    (* Always need to evaluate state, works more or less automatically *)
+    apply (simp add: STATE_interp_update_retrieve_key_eq_if)
+    subgoal sorry
+
+    using Rel_nat_Nil_nat (* Basic relations in simpset? *)
+    apply (simp add: STATE_interp_update_retrieve_key_eq_if)
+
+    apply (tactic \<open>SUT.STATE_interp_update_eq_STATE_interp_fun_upd (HOL_Nat_To_IMP_Tactics_Base.simp_update_tac @{context}) @{context} 1\<close>)
+
+    apply (tactic \<open>HT.run_step_tac HT.get_imp_minus_correct @{context} 1\<close>)
+    apply (tactic \<open>HT.run_step_tac HT.get_imp_minus_correct @{context} 1\<close>)
+    apply (tactic \<open>HT.run_step_tac HT.get_imp_minus_correct @{context} 1\<close>)
+    apply (tactic \<open>HT.run_step_tac HT.get_imp_minus_correct @{context} 1\<close>)
+    apply (tactic \<open>HT.run_step_tac HT.get_imp_minus_correct @{context} 1\<close>)
+    apply (tactic \<open>HT.run_step_tac HT.get_imp_minus_correct @{context} 1\<close>)
+    apply (tactic \<open>HT.run_step_tac HT.get_imp_minus_correct @{context} 1\<close>)
+     apply (tactic \<open>HT.finish_non_tail_tac @{context} 1\<close>)
+    (* Apply transfer \<rightarrow> find contradiction *)
+    subgoal
+      sorry
+
+    apply (tactic \<open>HT.run_step_tac HT.get_imp_minus_correct @{context} 1\<close>)
+    apply (tactic \<open>HT.run_step_tac HT.get_imp_minus_correct @{context} 1\<close>)
+    apply (tactic \<open>HT.run_step_tac HT.get_imp_minus_correct @{context} 1\<close>)
+    apply (tactic \<open>HT.run_step_tac HT.get_imp_minus_correct @{context} 1\<close>)
+    apply (tactic \<open>HT.run_step_tac HT.get_imp_minus_correct @{context} 1\<close>)
+    apply (tactic \<open>HT.run_step_tac HT.get_imp_minus_correct @{context} 1\<close>)
+    apply (tactic \<open>HT.run_step_tac HT.get_imp_minus_correct @{context} 1\<close>)
+    apply (tactic \<open>HT.run_step_tac HT.get_imp_minus_correct @{context} 1\<close>)
+    apply (tactic \<open>HT.finish_non_tail_tac @{context} 1\<close>)
+    (* Apply transfer *)
+
+    (* Stupid sledgehammer proof *)
+    by (smt (z3) Rel_nat_destruct_Cons(1) Rel_nat_suc_nat
+        \<open>\<And>ya. Rel_nat (s ''rev_test_nat.args.x'') (x # xs) \<Longrightarrow> fst_nat (s ''rev_test_nat.args.x'') \<noteq> 0 \<Longrightarrow> Rel_nat (Cons_nat (fst_nat (snd_nat (s ''rev_test_nat.args.x''))) (snd_nat (snd_nat (s ''rev_test_nat.args.x'')))) ya\<close>
+        left_uniqueD left_unique_Rel_nat n_not_Suc_n rel_funD)
   sorry
+
+
 
 end
 
@@ -214,84 +378,56 @@ context HOL_Nat_To_IMP_Minus
 begin
 
 lemmas length_acc_nat_eq = HTHN.length_acc_nat_eq_unfolded[simplified case_list_nat_def]
-unconditional_nat length_acc_nat_eq
-declare length_acc_nat_unconditional.simps[simp del]
-compile_nat length_acc_nat_unconditional.simps
-HOL_To_IMP_Minus_correct length_acc_nat_unconditional by (cook mode = tailcall)
+compile_nat length_acc_nat_eq
+HOL_To_IMP_Minus_correct HOL_To_HOL_Nat.length_acc_nat
+  oops
 
-lemma related_length_acc_nat_unconditional [transfer_rule]:
-  "(Rel_nat ===> Rel_nat ===> Rel_nat) length_acc_nat_unconditional HTHN.length_acc"
+lemma "Rel_nat (s ''length_acc_nat.args.x'') (y::'a list) \<Longrightarrow>
+       Rel_nat (s ''length_acc_nat.args.xa'') (ya::nat) \<Longrightarrow>
+    terminates_with_res_IMP_Minus (tailcall_to_IMP_Minus length_acc_nat_IMP_tailcall)
+      s ''length_acc_nat.ret''
+     (HTHN.length_acc_nat TYPE('a::compile_nat) (s ''length_acc_nat.args.x'') (s ''length_acc_nat.args.xa''))"
+  apply (rule terminates_with_res_IMP_Minus_if_terminates_with_res_IMP_TailcallI)
+    apply (subst length_acc_nat_IMP_tailcall_def; simp)
+  apply (subst length_acc_nat_IMP_tailcall_def; simp)
+  apply (induction "y" "ya" arbitrary: s rule: HTHN.length_acc.induct)
+  (*case []*)
+  apply (subst (2) length_acc_nat_IMP_tailcall_def, rule terminates_with_res_IMP_Tailcall_start)
+   apply (tactic \<open>HT.run_step_tac HT.get_imp_minus_correct @{context} 1\<close>)+
+    (*check the retrieved condition for a contradiction (needs to be built into the IF tactic*)
+    apply (erule check_first_nat_ccontradictionE check_first_nat_ccontradictionE')
+    apply (rule fst_nat_eq_if_Rel_nat_list)
+    apply assumption (*needs a smarter method*)
+    apply simp
+  apply (subst HTHN.length_acc_nat_eq_unfolded)
+  apply (assumption, assumption)
+  apply (subst case_list_nat_def)
+  apply (split if_splits; intro impI conjI; simp)
+  apply (tactic \<open>HT.finish_non_tail_tac @{context} 1\<close>)
+    (*we need to derive a contradiction*)
+    apply (erule check_first_nat_ccontradictionE check_first_nat_ccontradictionE')
+    apply (rule fst_nat_eq_if_Rel_nat_list)
+    apply assumption
+    apply simp
+  (*case x#xs*)
+  apply (subst (2) length_acc_nat_IMP_tailcall_def, rule terminates_with_res_IMP_Tailcall_start)
+  apply (tactic \<open>HT.run_step_tac HT.get_imp_minus_correct @{context} 1\<close>)+
+    (*we need to derive a contradiction*)
+    apply (erule check_first_nat_ccontradictionE check_first_nat_ccontradictionE')
+    apply (rule fst_nat_eq_if_Rel_nat_list)
+    apply assumption
+    apply simp
+    (*check the retrievied condition for a contradiction*)
+    apply (erule check_first_nat_ccontradictionE check_first_nat_ccontradictionE')
+    apply (rule fst_nat_eq_if_Rel_nat_list)
+    apply assumption
+    apply simp
+  apply (tactic \<open>HT.run_step_tac HT.get_imp_minus_correct @{context} 1\<close>)+
+  apply (subst HTHN.length_acc_nat_eq_unfolded)
+  apply (assumption, assumption)
+  apply (subst case_list_nat_def)
+  apply (split if_splits; intro impI conjI; simp)
   sorry
-
-end
-
-context HOL_To_HOL_Nat
-begin
-
-(*introduce a definition because List.length is just an abbreviation*)
-definition length where "length xs \<equiv> length_acc xs 0"
-
-lemma length_eq_length [simp]: "length = List.length"
-  unfolding length_def by simp
-
-declare HNTIM.related_length_acc_nat_unconditional[transfer_rule]
-function_compile_nat length_def
-
-end
-
-context HOL_Nat_To_IMP_Minus
-begin
-
-unconditional_nat HTHN.length_nat_eq_unfolded
-declare length_nat_unconditional.simps[simp del]
-compile_nat length_nat_unconditional.simps
-HOL_To_IMP_Minus_correct length_nat_unconditional by cook
-
-lemma related_length_nat_unconditional [transfer_rule]:
-  "(Rel_nat ===> Rel_nat) length_nat_unconditional length"
-  sorry
-
-end
-
-context HOL_To_HOL_Nat
-begin
-
-lemma append_eq_rev_acc_rev: "List.append xs ys = rev_acc (rev xs) ys"
-  by simp
-
-(*for some reason, transfer needs the lemma below instead of the existing, point-free version to
-synthesise the right definition*)
-(* declare HNTIM.related_rev_nat_unconditional[transfer_rule] *)
-
-lemma related_rev_nat_unconditional [transfer_rule]:
-  assumes "Rel_nat xs ys"
-  shows "Rel_nat (HNTIM.rev_nat_unconditional xs) (rev ys)"
-  by (fact rel_funD[OF HNTIM.related_rev_nat_unconditional assms])
-
-(* schematic_goal
-  assumes [transfer_rule]: "Rel_nat f xs"
-  assumes [transfer_rule]: "Rel_nat g ys"
-  shows "Rel_nat
-    (HNTIM.rev_acc_nat_unconditional (HNTIM.rev_nat_unconditional f) g)
-    (rev_acc (rev xs) ys)"
-  by transfer_prover *)
-
-function_compile_nat append_eq_rev_acc_rev
-
-end
-
-context HOL_Nat_To_IMP_Minus
-begin
-
-unconditional_nat HTHN.append_nat_eq_unfolded
-declare append_nat_unconditional.simps[simp del]
-compile_nat append_nat_unconditional.simps
-HOL_To_IMP_Minus_correct append_nat_unconditional by cook
-
-lemma related_append_nat_unconditional [transfer_rule]:
-  "(Rel_nat ===> Rel_nat ===> Rel_nat) append_nat_unconditional append"
-  sorry
-
 end
 
 context HOL_To_HOL_Nat
@@ -315,44 +451,227 @@ context HOL_Nat_To_IMP_Minus
 begin
 
 lemmas zip_acc_nat_eq = HTHN.zip_acc_nat_eq_unfolded[simplified case_list_nat_def]
-unconditional_nat zip_acc_nat_eq
-declare zip_acc_nat_unconditional.simps [simp del]
-compile_nat zip_acc_nat_unconditional.simps
-HOL_To_IMP_Minus_correct zip_acc_nat_unconditional by (cook mode = tailcall)
-
-lemma related_zip_acc_nat_unconditional [transfer_rule]:
-  "(Rel_nat ===> Rel_nat ===> Rel_nat ===> Rel_nat) zip_acc_nat_unconditional HTHN.zip_acc"
+compile_nat zip_acc_nat_eq
+HOL_To_IMP_Minus_correct HOL_To_HOL_Nat.zip_acc_nat
   sorry
 
+lemma "Rel_nat (s ''zip_acc_nat.args.x'') (y::'a list) \<Longrightarrow>
+    Rel_nat (s ''zip_acc_nat.args.xa'') (ya::'b list) \<Longrightarrow>
+    Rel_nat (s ''zip_acc_nat.args.xb'') (yb::('a * 'b) list) \<Longrightarrow>
+    terminates_with_res_IMP_Minus (tailcall_to_IMP_Minus zip_acc_nat_IMP_tailcall)
+      s ''zip_acc_nat.ret''
+     (HTHN.zip_acc_nat TYPE('a::compile_nat) TYPE('b::compile_nat)
+       (s ''zip_acc_nat.args.x'') (s ''zip_acc_nat.args.xa'') (s ''zip_acc_nat.args.xb''))"
+  apply (rule terminates_with_res_IMP_Minus_if_terminates_with_res_IMP_TailcallI)
+   apply (subst zip_acc_nat_IMP_tailcall_def; simp)
+   apply (subst zip_acc_nat_IMP_tailcall_def; simp)
+  apply (induction y ya yb arbitrary: s rule: HTHN.zip_acc.induct)
+  (*case [] _*)
+  apply (subst (2) zip_acc_nat_IMP_tailcall_def, rule terminates_with_res_IMP_Tailcall_start)
+  apply (tactic \<open>HT.run_step_tac HT.get_imp_minus_correct @{context} 1\<close>)+
+    (*check the retrieved condition for a contradiction (needs to be built into the IF tactic*)
+    apply (erule check_first_nat_ccontradictionE check_first_nat_ccontradictionE')
+    apply (rule fst_nat_eq_if_Rel_nat_list)
+    apply assumption (*needs a smarter method*)
+    apply simp
+  apply (subst HTHN.zip_acc_nat_eq_unfolded)
+    apply (assumption, assumption, assumption)
+    apply (subst case_list_nat_def)
+    apply (split if_splits; intro impI conjI; simp)
+    apply (tactic \<open>HT.finish_non_tail_tac @{context} 1\<close>)
+    (*we need to derive a contradiction*)
+    apply (erule check_first_nat_ccontradictionE check_first_nat_ccontradictionE')
+     apply (rule fst_nat_eq_if_Rel_nat_list)
+    apply assumption
+    apply simp
+  (* case _ []*)
+  apply (subst (2) zip_acc_nat_IMP_tailcall_def, rule terminates_with_res_IMP_Tailcall_start)
+   apply (tactic \<open>HT.run_step_tac HT.get_imp_minus_correct @{context} 1\<close>)+
+      (*check first case \<rightarrow> find contradiction*)
+    apply (erule check_first_nat_ccontradictionE check_first_nat_ccontradictionE')
+    apply (rule fst_nat_eq_if_Rel_nat_list)
+    apply assumption (*needs a smarter method*)
+    apply simp
+   apply (tactic \<open>HT.run_step_tac HT.get_imp_minus_correct @{context} 1\<close>)+
+    apply (erule check_first_nat_ccontradictionE check_first_nat_ccontradictionE')
+    apply (rule fst_nat_eq_if_Rel_nat_list)
+     apply assumption (*needs a smarter method*)
+  subgoal for v
+    sorry
+
+    (* Need to apply the search for contradiction multiple times ! *)
+    apply (erule check_first_nat_ccontradictionE check_first_nat_ccontradictionE')
+    apply (rule fst_nat_eq_if_Rel_nat_list)
+    apply assumption
+    apply (erule check_first_nat_ccontradictionE check_first_nat_ccontradictionE')
+    apply (rule fst_nat_eq_if_Rel_nat_list)
+    apply assumption
+    apply simp
+
+  (*case x#xs*)
+  apply (subst (2) zip_acc_nat_IMP_tailcall_def, rule terminates_with_res_IMP_Tailcall_start)
+  apply (tactic \<open>HT.run_step_tac HT.get_imp_minus_correct @{context} 1\<close>)+
+    (*we need to derive a contradiction*)
+    apply (erule check_first_nat_ccontradictionE check_first_nat_ccontradictionE')
+    apply (rule fst_nat_eq_if_Rel_nat_list)
+    apply assumption
+    apply simp
+  apply (tactic \<open>HT.run_step_tac HT.get_imp_minus_correct @{context} 1\<close>)+
+    (*check the retrievied condition for a contradiction*)
+    apply (erule check_first_nat_ccontradictionE check_first_nat_ccontradictionE')
+    apply (rule fst_nat_eq_if_Rel_nat_list)
+    apply assumption
+    apply (erule check_first_nat_ccontradictionE check_first_nat_ccontradictionE')
+    apply (rule fst_nat_eq_if_Rel_nat_list)
+    apply assumption
+    apply simp
+  apply (tactic \<open>HT.run_step_tac HT.get_imp_minus_correct @{context} 1\<close>)+
+    subgoal for v
+      sorry
+    done
+
 end
+
 
 context HOL_To_HOL_Nat
 begin
 
-lemma zip_eq_rev_zip_acc_nil: "List.zip xs ys = rev (zip_acc xs ys [])"
-  by simp
+fun count_acc :: "'a \<Rightarrow> 'a list \<Rightarrow> nat \<Rightarrow> nat" where
+  "count_acc a [] n = n"
+| "count_acc a (x#xs) n = (if x = a then count_acc a xs (Suc n) else count_acc a xs n)"
+declare count_acc.simps[simp del]
 
-(*TODO: why is this needed?*)
-declare
-  HNTIM.related_zip_acc_nat_unconditional[THEN rel_funD, THEN rel_funD, THEN rel_funD,transfer_rule]
-
-(*TODO: something is quite slow here*)
-function_compile_nat zip_eq_rev_zip_acc_nil
+case_of_simps count_acc_eq : count_acc.simps
+function_compile_nat count_acc_eq
 
 end
 
 context HOL_Nat_To_IMP_Minus
 begin
 
-unconditional_nat HTHN.zip_nat_eq_unfolded
-declare zip_nat_unconditional.simps [simp del]
-compile_nat zip_nat_unconditional.simps
-HOL_To_IMP_Minus_correct zip_nat_unconditional by cook
+lemmas count_acc_nat_eq = HTHN.count_acc_nat_eq_unfolded[simplified case_list_nat_def]
+compile_nat count_acc_nat_eq
+HOL_To_IMP_Minus_correct HOL_To_HOL_Nat.count_acc_nat
+  oops
 
-lemma related_zip_nat_unconditional [transfer_rule]:
-  "(Rel_nat ===> Rel_nat ===> Rel_nat) zip_nat_unconditional List.zip"
-  sorry
+lemma count_acc_cor: "Rel_nat (s ''count_acc_nat.args.x'') (y::'a) \<Longrightarrow>
+    Rel_nat (s ''count_acc_nat.args.xa'') (ya::'a list) \<Longrightarrow>
+    Rel_nat (s ''count_acc_nat.args.xb'') (yb::nat) \<Longrightarrow>
+    terminates_with_res_IMP_Minus
+     (tailcall_to_IMP_Minus count_acc_nat_IMP_tailcall) s
+     ''count_acc_nat.ret''
+     (HTHN.count_acc_nat TYPE('a::compile_nat)
+       (s ''count_acc_nat.args.x'')
+       (s ''count_acc_nat.args.xa'')
+       (s ''count_acc_nat.args.xb''))"
+  apply (rule terminates_with_res_IMP_Minus_if_terminates_with_res_IMP_TailcallI)
+   apply (subst count_acc_nat_IMP_tailcall_def; simp)
+   apply (subst count_acc_nat_IMP_tailcall_def; simp)
+  apply (induction y ya yb arbitrary: s rule: HTHN.count_acc.induct)
+  (* case [] *)
+  apply (subst (2) count_acc_nat_IMP_tailcall_def, rule terminates_with_res_IMP_Tailcall_start)
+  apply (tactic \<open>HT.run_step_tac HT.get_imp_minus_correct @{context} 1\<close>)+
+    (* correct case *)
+    apply (subst HTHN.count_acc_nat_eq_unfolded)
+    apply (assumption, assumption, assumption)
+    apply (subst case_list_nat_def)
+    apply (split if_splits; intro impI conjI; simp)
+    apply (tactic \<open>HT.finish_non_tail_tac @{context} 1\<close>)
+    (* wrong case *)
+    apply (erule check_first_nat_ccontradictionE check_first_nat_ccontradictionE')
+    apply (rule fst_nat_eq_if_Rel_nat_list)
+    apply assumption
+    apply simp
+  (* case x#xs *)
+  apply (subst (2) count_acc_nat_IMP_tailcall_def, rule terminates_with_res_IMP_Tailcall_start)
+  apply (tactic \<open>HT.run_step_tac HT.get_imp_minus_correct @{context} 1\<close>)+
+    apply (erule check_first_nat_ccontradictionE check_first_nat_ccontradictionE')
+    apply (rule fst_nat_eq_if_Rel_nat_list)
+    apply assumption
+    apply simp
+  apply (tactic \<open>HT.run_step_tac HT.get_imp_minus_correct @{context} 1\<close>)+
+    apply (subst HTHN.count_acc_nat_eq_unfolded)
+    apply (assumption, assumption, assumption)
+    apply (subst case_list_nat_def)
+    apply (split if_splits; intro impI conjI; simp)
+    subgoal for v
+    sorry
+  apply (tactic \<open>HT.run_step_tac HT.get_imp_minus_correct @{context} 1\<close>)+
+    apply (subst HTHN.count_acc_nat_eq_unfolded)
+    apply (assumption, assumption, assumption)
+    apply (subst case_list_nat_def)
+    apply (split if_splits; intro impI conjI; simp)
+    subgoal for v
+    sorry
+  done
+
+HOL_To_IMP_Minus_correct HOL_To_HOL_Nat.count_acc_nat
+  using count_acc_cor by blast
 
 end
+
+
+context HOL_To_HOL_Nat
+begin
+
+fun count_acc2 :: "'a \<Rightarrow> 'a list \<Rightarrow> nat \<Rightarrow> nat" where
+  "count_acc2 a [] n = n"
+| "count_acc2 a (x#xs) n = count_acc2 a xs (if x = a then Suc n else n)"
+declare count_acc2.simps[simp del]
+
+case_of_simps count_acc2_eq : count_acc2.simps
+function_compile_nat count_acc2_eq
+
+end
+
+context HOL_Nat_To_IMP_Minus
+begin
+
+lemmas count_acc2_nat_eq = HTHN.count_acc2_nat_eq_unfolded[simplified case_list_nat_def]
+compile_nat count_acc2_nat_eq
+HOL_To_IMP_Minus_correct HOL_To_HOL_Nat.count_acc2_nat
+  oops
+
+lemma count_acc2_cor: "Rel_nat (s ''count_acc2_nat.args.x'') (y::'a) \<Longrightarrow>
+    Rel_nat (s ''count_acc2_nat.args.xa'') (ya::'a list) \<Longrightarrow>
+    Rel_nat (s ''count_acc2_nat.args.xb'') (yb::nat) \<Longrightarrow>
+    terminates_with_res_IMP_Minus
+     (tailcall_to_IMP_Minus count_acc2_nat_IMP_tailcall) s
+     ''count_acc2_nat.ret''
+     (HTHN.count_acc2_nat TYPE('a::compile_nat)
+       (s ''count_acc2_nat.args.x'')
+       (s ''count_acc2_nat.args.xa'')
+       (s ''count_acc2_nat.args.xb''))"
+  apply (rule terminates_with_res_IMP_Minus_if_terminates_with_res_IMP_TailcallI)
+   apply (subst count_acc2_nat_IMP_tailcall_def; simp)
+   apply (subst count_acc2_nat_IMP_tailcall_def; simp)
+  apply (induction y ya yb arbitrary: s rule: HTHN.count_acc.induct)
+  (* case [] *)
+  apply (subst (2) count_acc2_nat_IMP_tailcall_def, rule terminates_with_res_IMP_Tailcall_start)
+  apply (tactic \<open>HT.run_step_tac HT.get_imp_minus_correct @{context} 1\<close>)+
+    (* correct case *)
+    apply (subst HTHN.count_acc2_nat_eq_unfolded)
+    apply (assumption, assumption, assumption)
+    apply (subst case_list_nat_def)
+    apply (split if_splits; intro impI conjI; simp)
+    apply (tactic \<open>HT.finish_non_tail_tac @{context} 1\<close>)
+    (* wrong case *)
+    apply (erule check_first_nat_ccontradictionE check_first_nat_ccontradictionE')
+    apply (rule fst_nat_eq_if_Rel_nat_list)
+    apply assumption
+    apply simp
+  (* case x#xs *)
+  apply (subst (2) count_acc2_nat_IMP_tailcall_def, rule terminates_with_res_IMP_Tailcall_start)
+  apply (tactic \<open>HT.run_step_tac HT.get_imp_minus_correct @{context} 1\<close>)+
+    apply (erule check_first_nat_ccontradictionE check_first_nat_ccontradictionE')
+    apply (rule fst_nat_eq_if_Rel_nat_list)
+    apply assumption
+    apply simp
+  apply (tactic \<open>HT.run_step_tac HT.get_imp_minus_correct @{context} 1\<close>)+
+  sorry
+
+HOL_To_IMP_Minus_correct HOL_To_HOL_Nat.count_acc2_nat
+  using count_acc2_cor by blast
+
 
 end
